ground_zero/HITs/interval.lean
@@ -1,5 +1,7 @@
-import ground_zero.HITs.trunc
-open ground_zero.HITs.trunc ground_zero.structures
+import ground_zero.HITs.generalized ground_zero.structures
+open ground_zero.HITs ground_zero.structures
+
+hott theory
 
 /-
   The unit interval I as Higher Inductive Type.
@@ -13,15 +15,21 @@ open ground_zero.HITs.trunc ground_zero.structures
 namespace ground_zero
 namespace HITs
 
-def I := ∥bool∥
+notation [parsing_only] `𝟐` := bool
+
+def I := {𝟐}
 abbreviation interval := I
 
 namespace interval
   universes u v
 
-  def i₀ : I := trunc.elem ff
-  def i₁ : I := trunc.elem tt
-  def seg : i₀ = i₁ :> I := trunc.uniq i₀ i₁
+  def i₀ : I := generalized.incl ff
+  def i₁ : I := generalized.incl tt
+
+  def seg : i₀ = i₁ := generalized.glue ff tt
+  def seg_inv : i₁ = i₀ := generalized.glue tt ff
+
+  def discrete : bool → I := generalized.incl
 
   instance : has_zero I := ⟨i₀⟩
   instance : has_one I := ⟨i₁⟩
@@ -37,8 +45,10 @@ namespace interval
     (s : b₀ = b₁ :> β) : I → β :=
   let f (b : bool) : singl b₀ :=
     bool.rec (singl.trivial_loop b₀) ⟨b₁, s⟩ b in
-  singl.point ∘ trunc.rec (structures.contr_impl_prop $
-    singl.signl_contr b₀) f
+  singl.point ∘ generalized.rec f (begin intros, apply singl.singl_prop end)
+
+  def lift {β : Sort u} (f : bool → β) (H : prop β) : I → β :=
+  generalized.rec f (begin intros, apply H end)
 
   /- β i₀ and β i₁ are Prop’s,
      so s : b₀ = b₁ is trivial -/
@@ -51,7 +61,7 @@ namespace interval
   def hrec (β : I → Sort u)
     (b₀ : β 0) (b₁ : β 1) (s : b₀ == b₁)
     (x : I) : β x :=
-  @quot.hrec_on bool (λ _ _, true) β x
+  quot.hrec_on x
     (λ i, bool.rec_on i b₀ b₁)
     (λ a b _,
       begin simp, induction a; induction b; simp,
@@ -70,6 +80,20 @@ namespace interval
       { reflexivity } }
   end
 
+  def interval_contr : contr I := begin
+    existsi i₁,
+    fapply ind,
+    { exact seg⁻¹ }, { reflexivity },
+    { apply types.equiv.pathover_from_trans,
+      apply types.eq.inv_comp }
+  end
+
+  def interval_prop : prop I :=
+  contr_impl_prop interval_contr
+
+  def seg_inv_comp : seg ⬝ seg⁻¹ = types.eq.rfl :=
+  by apply prop_is_set interval_prop
+
   def homotopy {α : Sort u} {β : Sort v} {f g : α → β}
     (p : f ~ g) (x : α) : I → β :=
   rec (f x) (g x) (p x)
@@ -86,29 +110,24 @@ namespace interval
   in lem # seg
 
   def homotopy_from_path {α : Sort u} {β : α → Sort v}
-    {f g : Π (x : α), β x} (p : f = g :> _) : f ~ g :=
+    {f g : Π (x : α), β x} (p : f = g) : f ~ g :=
   begin induction p, apply types.equiv.homotopy.id end
 
-  def interval_prop : prop I := trunc.uniq
-  def trunc_functions {α : Type u} : prop (∥α∥ → ∥α∥) :=
-  begin intros x y, apply funext, intro x, apply trunc.uniq end
-
   def neg : I → I :=
-  trunc.rec interval_prop (trunc.elem ∘ bnot)
+  lift (discrete ∘ bnot) interval_prop
   prefix `−`:80 := neg
   instance : has_neg I := ⟨neg⟩
 
   def bool_to_interval (f : bool → bool → bool) (a b : I) : I :=
-  trunc.rec interval_prop (λ a,
-    trunc.rec interval_prop (trunc.elem ∘ f a) b) a
+  lift (λ a, lift (discrete ∘ f a) interval_prop b) interval_prop a
 
   def min (a b : I) : I :=
-  trunc.rec interval_prop (begin
-    intro x, cases x, exact i₀, exact a end) b
+  lift (begin intro x, cases x, exact i₀, exact a end)
+        interval_prop b
 
   def max (a b : I) : I :=
-  trunc.rec interval_prop (begin
-    intro x, cases x, exact a, exact i₁ end) b
+  lift (begin intro x, cases x, exact a, exact i₁ end)
+        interval_prop b
 
   notation r `∧`:70 s := min r s
   notation r `∨`:70 s := max r s
