ground_zero/theorems/mere_eq_lemma.lean
@@ -1,20 +1,20 @@
-import ground_zero.HITs.trunc
+import ground_zero.HITs.truncation
 open ground_zero
 
 namespace ground_zero.mere_eq_lemma
 universe u
 
 def to_mere_eq {α β : Sort u} (h : α = β) : ∥α = β :> Sort u∥ :=
-begin induction h, apply ground_zero.HITs.trunc.elem, reflexivity end
+begin induction h, apply ground_zero.HITs.truncation.elem, reflexivity end
 
 def from_mere_eq {α β : Sort u} : ∥α = β :> Sort u∥ → α = β :=
-HITs.trunc.rec structures.prop_impl_prop
+HITs.truncation.rec structures.prop_impl_prop
   (begin intro x, induction x, reflexivity end)
 
 lemma mere_eq {α β : Sort u} : (α = β) ≃ ∥α = β :> Sort u∥ := begin
   existsi to_mere_eq, split; existsi from_mere_eq,
   { trivial },
-  { intro h, simp, apply HITs.trunc.uniq }
+  { intro h, simp, apply HITs.truncation.uniq }
 end
 
 end ground_zero.mere_eq_lemma
